wip

src/Minimal.Hardware.fst
@@ -1,10 +1,5 @@
 module Minimal.Hardware
 
-open Lib.IntTypes
-
-open Spec.Hash.Definitions
-open Hacl.Hash.Definitions
-
 module P = FStar.Preorder
 module G = FStar.Ghost
 
@@ -14,48 +9,15 @@ module HST = FStar.HyperStack.ST
 module B = LowStar.Buffer
 
 let uds_len = 0x20ul
-let header_len = 0x20ul
-let entry_t = unit -> HST.St unit
-let entry = fun () -> ()
 
-noeq
-type header_t = {
-     (* actual entries in headers*)
-     binary_size   : binary_size_t;
-     binary_hash   : digest_t;
-     header_sig    : signature_t;
-     (* extra entries for convenience *)
-     binary        : B.lbuffer uint8 (v binary_size);
-     header_raw    : header_raw_t;
-     header_pubkey : publickey_t;
-     entry         : entry_t;
-     header_inv    : u:unit{
-       B.(all_disjoint [ loc_buffer binary_hash
-                       ; loc_buffer header_sig
-                       ; loc_buffer binary
-                       ; loc_buffer header_raw
-                       ; loc_buffer header_pubkey ] /\
-       length binary == v binary_size)
-     }
-}
+#set-options "--max_fuel 0 --ifuel 2"
 
-let get_binary_size header = header.binary_size
-let get_binary_hash header = header.binary_hash
-let get_header_sig  header = header.header_sig
-let get_binary      header = header.binary
-let get_header_raw  header = header.header_raw
-let get_header_pubkey header = header.header_pubkey
-let get_entry       header = header.entry
-
-/// <><><><><><><><><><><><> Monotonic Predicates <><><><><><><><><><><><>
-/// 
-noextract
 type t =
   | Uninitialized
   | Enabled
   | Disabled
 
-noextract
+
 let t_rel : P.preorder (G.erased t) =
   fun x1 x2 ->
   match (G.reveal x1, G.reveal x2) with
@@ -63,105 +25,91 @@ let t_rel : P.preorder (G.erased t) =
   | Enabled, Disabled -> True
   | _, _ -> x1 == x2
 
-noextract
+
 let local_state_ref : HST.mref (G.erased t) t_rel = HST.ralloc HS.root (G.hide Uninitialized)
 
+
 let local_state = (| t, t_rel,  local_state_ref |)
+
 
 let uds_is_uninitialized h =
   G.reveal (HS.sel h local_state_ref) == Uninitialized
 
-noextract
+
 let uds_is_initialized_predicate : HST.mem_predicate =
   fun h ->
   let x = G.reveal (HS.sel h local_state_ref) in
   x == Enabled \/ x == Disabled
 
+
 let uds_is_initialized = HST.token_p local_state_ref uds_is_initialized_predicate
 
-noextract
+
 let uds_is_disabled_predicate : HST.mem_predicate =
   fun h -> G.reveal (HS.sel h local_state_ref) == Disabled
 
+
 let uds_is_disabled = HST.token_p local_state_ref uds_is_disabled_predicate
 
-/// <><><><><><><><><><><><><><><><> State <><><><><><><><><><><><><><><><>
 
 noeq
 type state = {
-  uds     : B.buffer uint8;
-  cdi     : B.buffer uint8;
-  header  : header_t;
+  uds : B.buffer uint8;
+  cdi : B.buffer uint8;
+  riot_header : riot_header_t;
   uds_val : s:G.erased (Seq.seq uint8){
     B.length uds == v uds_len /\
     B.length cdi == v cdi_len /\
     Seq.length (G.reveal s) == v uds_len /\
     B.freeable uds /\
     B.freeable cdi /\
-    B.all_disjoint ([B.loc_buffer uds
-                   ; B.loc_buffer cdi
-                   ; B.loc_mreference local_state_ref] @
-                   (get_header_loc_l header))
-  }
+    B.all_disjoint ([
+      B.loc_buffer uds;
+      B.loc_buffer cdi;
+      B.loc_mreference local_state_ref;
+      B.loc_buffer riot_header.binary_hash;
+      B.loc_buffer riot_header.header_sig;
+      B.loc_buffer riot_header.binary;
+      B.loc_buffer riot_header.pubkey])
+  };
 }
+
 
 let get_uds st = st.uds
 let get_cdi st = st.cdi
-let get_header st = st.header
 let get_uds_value st = G.reveal st.uds_val
+let get_riot_header st = st.riot_header
 
-let load_header
-  (_: unit)
-: HST.ST (header: header_t)
-  (requires fun h -> True)
-  (ensures fun h0 header h1 -> True)
-=
-  let binary_size:binary_size_t   = 100ul in
-  let binary_hash   = B.malloc HS.root (u8 0x00) digest_len in
-  let header_sig    = B.malloc HS.root (u8 0x00) 64ul in
-  let binary        = B.malloc HS.root (u8 0x00) binary_size in
-  let header_raw    = B.malloc HS.root (u8 0x00) header_len in
-  let header_pubkey = B.malloc HS.root (u8 0x00) 32ul in
-  { binary_size = binary_size
-  ; binary_hash = binary_hash
-  ; header_sig  = header_sig
-  ; binary      = binary
-  ; header_raw  = header_raw
-  ; header_pubkey = header_pubkey
-  ; entry       = entry
-  ; header_inv  = () }
-
-#reset-options "--z3rlimit 50"
-#push-options "--query_stats"
 let initialize () =
   HST.recall local_state_ref;
   HST.(local_state_ref := Enabled);
   HST.witness_p local_state_ref uds_is_initialized_predicate;
 
   let uds = B.malloc HS.root (u8 0x00) uds_len in
-  let cdi = B.malloc HS.root (u8 0x00) uds_len in
-  let binary_size   = 100ul in
-  let binary_hash   = B.malloc HS.root (u8 0x00) digest_len in
-  let header_sig    = B.malloc HS.root (u8 0x00) 64ul in
-  let binary        = B.malloc HS.root (u8 0x00) binary_size in
-  let header_raw    = B.malloc HS.root (u8 0x00) header_len in
-  let header_pubkey = B.malloc HS.root (u8 0x00) 32ul in
+  let cdi = B.malloc HS.root (u8 0x00) cdi_len in
+
+  let binary_size = 1ul in
+  let binary_hash = B.malloc HS.root (u8 0x00) digest_len in
+  let header_sig = B.malloc HS.root (u8 0x00) 64ul in
+  let binary = B.malloc HS.root (u8 0x00) 1ul in
+  let pubkey = B.malloc HS.root (u8 0x00) 32ul in
+
+  let riot_header = {
+    binary_size = binary_size;
+    binary_hash = binary_hash;
+    header_sig = header_sig;
+    binary = binary;
+    pubkey = pubkey
+  } in
 
   let uds_seq =
     let h = HST.get () in
     G.hide (B.as_seq h uds) in
 
-  { uds = uds
-  ; cdi = cdi
-  ; header  = { binary_size = binary_size
-              ; binary_hash = binary_hash
-              ; header_sig  = header_sig
-              ; binary      = binary
-              ; header_raw  = header_raw
-              ; header_pubkey = header_pubkey
-              ; entry       = entry
-              ; header_inv  = () }
-  ; uds_val = uds_seq }
+  { uds = uds;
+    cdi = cdi;
+    riot_header = riot_header;
+    uds_val = uds_seq }
 
 let unset_uds st =
   let uds = get_uds st in
