src/DICE.Definitions.fst
@@ -1,0 +1,78 @@
+module DICE.Definitions
+
+module HS = FStar.HyperStack
+
+module I = Lib.IntTypes
+module B = LowStar.Buffer
+
+module S = Spec.Hash.Definitions
+module H = Hacl.Hash.Definitions
+
+
+type dice_hash_alg = a:S.hash_alg{a =!= S.MD5 /\ a =!= S.SHA2_224}
+
+inline_for_extraction
+let alg : dice_hash_alg = S.SHA2_256
+
+inline_for_extraction noextract
+let dice_hash (alg:dice_hash_alg) : H.hash_st alg =
+  match alg with
+  | S.SHA2_256 -> Hacl.Hash.SHA2.hash_256
+  | S.SHA2_384 -> Hacl.Hash.SHA2.hash_384
+  | S.SHA2_512 -> Hacl.Hash.SHA2.hash_512
+  | S.SHA1     -> Hacl.Hash.SHA1.legacy_hash
+
+inline_for_extraction noextract
+let dice_hmac (alg:dice_hash_alg) : Hacl.HMAC.compute_st alg =
+  match alg with
+  | S.SHA2_256 -> Hacl.HMAC.compute_sha2_256
+  | S.SHA2_384 -> Hacl.HMAC.compute_sha2_384
+  | S.SHA2_512 -> Hacl.HMAC.compute_sha2_512
+  | S.SHA1     -> Hacl.HMAC.legacy_compute_sha1
+
+unfold let digest_len = H.hash_len alg
+
+unfold let digest_t = H.hash_t alg
+
+unfold let max_input_len = S.max_input_length alg
+
+unfold let hashable_len = i:I.size_t{0 < I.v i /\ I.v i <= max_input_len}
+
+unfold let signature_t = B.lbuffer I.uint8 64
+unfold let key_t = B.lbuffer I.uint8 32
+
+
+unfold let cdi_len = digest_len
+
+
+
+noeq
+type riot_header_t = {
+  binary_size : hashable_len;
+  binary_hash : digest_t;
+  header_sig  : signature_t;
+  
+  binary      : B.lbuffer I.uint8 (I.v binary_size);
+  pubkey      : (k:key_t{
+    B.(all_disjoint [
+        B.loc_buffer binary_hash;
+        B.loc_buffer header_sig;
+        B.loc_buffer binary;
+        B.loc_buffer k ])
+  });
+}
+
+let riot_header_locs (rh:riot_header_t) : GTot (list B.loc) = [
+  B.loc_buffer rh.binary_hash;
+  B.loc_buffer rh.header_sig;
+  B.loc_buffer rh.binary;
+  B.loc_buffer rh.pubkey
+]
+
+let contains_riot_header (h:HS.mem) (rh:riot_header_t) =
+  B.all_live h [
+    B.buf rh.binary_hash;
+    B.buf rh.header_sig;
+    B.buf rh.binary;
+    B.buf rh.pubkey
+  ]
